Update term definitions

Semantic/CC/Syntax/Exp.lean
@@ -8,19 +8,25 @@ namespace CC
 
 inductive Exp : Sig -> Type where
 | var : Var .var s -> Exp s
-| abs : Ty .shape s -> Exp (s,x) -> Exp s
+| abs : Ty .capt s -> Exp (s,x) -> Exp s
 | tabs : Ty .shape s -> Exp (s,X) -> Exp s
+| cabs : Exp (s,C) -> Exp s
 | app : Var .var s -> Var .var s -> Exp s
 | tapp : Var .var s -> Ty .shape s -> Exp s
+| capp : Var .var s -> CaptureSet s -> Exp s
 | letin : Exp s -> Exp (s,x) -> Exp s
+| unpack : Exp s -> Exp ((s,C),X) -> Exp s
 
 def Exp.rename : Exp s1 -> Rename s1 s2 -> Exp s2
 | .var x, f => .var (x.rename f)
 | .abs T e, f => .abs (T.rename f) (e.rename (f.lift))
 | .tabs T e, f => .tabs (T.rename f) (e.rename (f.lift))
+| .cabs e, f => .cabs (e.rename (f.lift))
 | .app x y, f => .app (x.rename f) (y.rename f)
 | .tapp x T, f => .tapp (x.rename f) (T.rename f)
+| .capp x cs, f => .capp (x.rename f) (cs.rename f)
 | .letin e1 e2, f => .letin (e1.rename f) (e2.rename (f.lift))
+| .unpack e1 e2, f => .unpack (e1.rename f) (e2.rename (f.lift.lift))
 
 inductive Exp.IsVal : Exp s -> Prop where
 | abs : Exp.IsVal (.abs T e)
@@ -37,7 +43,9 @@ def Exp.rename_id {e : Exp s} : e.rename (Rename.id) = e := by
   induction e
     <;> try (solve
       | rfl
-      | simp [Exp.rename, Ty.rename_id, Var.rename_id, Rename.lift_id]; try aesop)
+      | simp [Exp.rename, Ty.rename_id, Var.rename_id,
+              CaptureSet.rename_id, Rename.lift_id]
+        try aesop)
 
 theorem Var.rename_comp {x : Var k s1} {f : Rename s1 s2} {g : Rename s2 s3} :
     (x.rename f).rename g = x.rename (f.comp g) := by
@@ -48,7 +56,9 @@ theorem Exp.rename_comp {e : Exp s1} {f : Rename s1 s2} {g : Rename s2 s3} :
   induction e generalizing s2 s3
     <;> try (solve
       | rfl
-      | simp [Exp.rename, Ty.rename_comp, Var.rename_comp, Rename.lift_comp]; try aesop)
+      | simp [Exp.rename, Ty.rename_comp, Var.rename_comp,
+              CaptureSet.rename_comp, Rename.lift_comp]
+        try aesop)
 
 theorem Var.weaken_rename_comm {x : Var k s1} {f : Rename s1 s2} :
     (x.rename Rename.succ).rename (f.lift (k:=k0)) = (x.rename f).rename (Rename.succ) := by
